MirrorCharge!/src/Imp/STacCancelEx.v
@@ -1,0 +1,193 @@
+Require Import MirrorCore.Lambda.Expr.
+Require Import MirrorCore.STac.STac.
+Require MirrorCore.syms.SymEnv.
+Require MirrorCore.syms.SymSum.
+Require Import MirrorCore.Lambda.ExprUnify_simul.
+Require Import MirrorCharge.ILogicFunc.
+Require Import MirrorCharge.OrderedCanceller.
+Require Import MirrorCharge.BILNormalizeEx.
+Require Import MirrorCharge.SynSepLog.
+Require Import MirrorCharge.SepLogFold.
+Require Import MirrorCharge.Imp.Syntax.
+Require Import MirrorCore.Subst.CascadeSubst.
+
+Set Implicit Arguments.
+Set Strict Implicit.
+
+Local Existing Instance SS.
+Local Existing Instance SU.
+Local Existing Instance RSym_ilfunc.
+Local Existing Instance RS.
+Local Existing Instance Expr_expr.
+
+(** NOTE: this is for [locals -> HProp] **)
+Definition sls : SepLogFoldEx.SepLogSpec typ func :=
+{| SepLogFoldEx.is_pure := fun (e : expr typ func) =>
+                match e with
+                  | Inj (inr (ilf_true _))
+                  | Inj (inr (ilf_false _)) => true
+                  | _ => false
+                end
+ ; SepLogFoldEx.is_emp := fun e => false
+ ; SepLogFoldEx.is_star := fun (e : expr typ func) =>
+                match e with
+                  | Inj (inl (inr (pStar _))) => true
+                  | _ => false
+                end
+ ; SepLogFoldEx.is_and := fun (e : expr typ func) =>
+                match e with
+                  | Inj (inr (ilf_and _)) => true
+                  | _ => false
+                end
+ ; SepLogFoldEx.is_ex := fun (e : expr typ func) =>
+                match e with
+                  | Inj (inr (ilf_exists t _)) => Some t
+                  | _ => None
+                end
+ |}.
+
+Require Import MirrorCore.Lambda.ExprLift.
+
+Section inst_2.
+  Variable lookup : uvar -> nat -> option (expr typ func).
+
+  Fixpoint instantiate (u : nat) (e : expr typ func)
+  : expr typ func :=
+    match e with
+      | Var _ => e
+      | Inj _ => e
+      | App l r => App (instantiate u l) (instantiate u r)
+      | Abs t e =>
+        Abs t (instantiate (S u) e)
+      | UVar uv =>
+        match lookup uv u with
+          | None => UVar uv
+          | Some e => e
+        end
+    end.
+
+  Variable check : uvar -> bool.
+  Fixpoint mentions_any (e : expr typ func) : bool :=
+    match e with
+      | Var _ => false
+      | Inj _ => false
+      | App l r => if mentions_any l then true else mentions_any r
+      | Abs t e => mentions_any e
+      | UVar uv => check uv
+    end.
+End inst_2.
+
+Let Subst_CS : SubstI3.Subst (CascadeSubst subst subst) (expr typ func) :=
+  @Subst_CascadeSubst (expr typ func) subst _ subst _ (@lift typ func 0).
+Let SubstU_CS : SubstI3.SubstUpdate (CascadeSubst subst subst) (expr typ func) :=
+  @SubstUpdate_CascadeSubst (expr typ func) subst _ _ subst _
+                            (@lift typ func 0)
+                            (@lower typ func 0)
+                            mentions_any
+                            instantiate.
+Local Existing Instance Subst_CS.
+Local Existing Instance SubstU_CS.
+
+Let doUnifySepLog (tus tvs : EnvI.tenv typ) (s : CascadeSubst subst subst) (e1 e2 : expr typ func)
+: option (CascadeSubst subst subst) :=
+  @exprUnify _ typ func _ _ _ _ _ 10 nil tus tvs 0 s e1 e2 tyLProp.
+
+Let ssl : SynSepLog typ func :=
+{| e_star := fun l r =>
+               match l with
+                 | Inj (inl (inr (pEmp _))) => r
+                 | _ => match r with
+                          | Inj (inl (inr (pEmp _))) => l
+                          | _ => lstar tyLProp l r
+                        end
+               end
+ ; e_emp := lemp tyLProp
+ ; e_and := fun l r =>
+              match l with
+                | Inj (inr (ilf_true _)) => r
+                | _ => match r with
+                         | Inj (inr (ilf_true _)) => l
+                         | _ => land tyLProp l r
+                       end
+              end
+ ; e_true := ltrue tyLProp
+ |}.
+
+Definition eproveTrue (s : CascadeSubst subst subst) (e : expr typ func)
+: option (CascadeSubst subst subst) :=
+  match e with
+    | Inj (inr (ilf_true _)) => Some s
+    | _ => None
+  end.
+
+Definition is_solved (e1 e2 : BILNormalize.conjunctives typ func) : bool :=
+  match e1 , e2 with
+    | {| BILNormalize.spatial := e1s
+       ; BILNormalize.star_true := t
+       ; BILNormalize.pure := _ |}
+    , {| BILNormalize.spatial := nil
+       ; BILNormalize.star_true := t'
+       ; BILNormalize.pure := nil |} =>
+      if t' then
+        (** ... |- true **)
+        true
+      else
+        (** ... |- emp **)
+        if t then false else match e1s with
+                               | nil => true
+                               | _ => false
+                             end
+    | _ , _ => false
+  end.
+
+Definition the_canceller tus tvs (lhs rhs : expr typ func)
+           (s : subst)
+: (expr typ func * expr typ func * subst) + subst:=
+  match @normalize typ _ sls lhs
+      , @normalize typ _ sls rhs
+  with
+    | Some lhs_norm , Some rhs_norm =>
+      (** TODO: I need to build a new substitution **)
+      let s' := @over subst subst s (@SubstI3.empty _ _ _) (length tus) (length lhs_norm.(exs)) in
+      let '(lhs',rhs',s') :=
+          @OrderedCanceller.ordered_cancel
+            typ func (CascadeSubst subst subst)
+            (doUnifySepLog tus tvs) eproveTrue
+            (simple_order (func:=func))
+            {| BILNormalize.spatial := lhs_norm.(spatial)
+             ; BILNormalize.pure := lhs_norm.(pure)
+             ; BILNormalize.star_true := lhs_norm.(star_true) |}
+            {| BILNormalize.spatial := rhs_norm.(spatial)
+             ; BILNormalize.pure := rhs_norm.(pure)
+             ; BILNormalize.star_true := rhs_norm.(star_true) |}
+            s'
+      in
+      match SubstI3.pull (length tus) (length lhs_norm.(exs)) s' with
+        | None => inl (lhs, rhs, s)
+        | Some s' =>
+          if is_solved lhs' rhs' then
+            inr (s'.(lowerSubst))
+          else
+            (*inl (conjunctives_to_expr ssl lhs',
+                 conjunctives_to_expr ssl rhs',
+                 s') *)
+            inl (lhs, rhs, s)
+      end
+    | _ , _ => inl (lhs, rhs, s)
+  end.
+
+Definition stac_cancel (thn : stac typ (expr typ func) subst)
+: stac typ (expr typ func) subst :=
+  fun e s tus tvs =>
+    match e with
+      | App (App (Inj (inr (ilf_entails (tyArr tyLocals tyHProp)))) L) R =>
+        match the_canceller tus tvs L R s with
+          | inl (l,r,s') =>
+            let e' :=
+                App (App (Inj (inr (ilf_entails (tyArr tyLocals tyHProp)))) l) r
+            in
+            thn e' s tus tvs
+          | inr s' => @Solve _ _ _ s'
+        end
+      | _ => thn e s tus tvs
+    end.
