MirrorCharge!/src/SepLogFoldEx.v
@@ -1,0 +1,406 @@
+(** This file implements an interface to [expr] that
+ ** makes star, emp, and pure assertions apparent.
+ **)
+Require Import ExtLib.Data.Fun.
+Require Import ExtLib.Data.List.
+Require Import ExtLib.Data.Option.
+Require Import ExtLib.Structures.Traversable.
+Require Import ExtLib.Tactics.
+Require Import BILogic Pure.
+Require Import MirrorCore.EnvI.
+Require Import MirrorCore.SymI.
+Require Import MirrorCore.TypesI.
+Require Import MirrorCore.ExprI.
+Require Import MirrorCore.Lambda.Expr.
+Require Import MirrorCore.Lambda.AppN.
+Require Import MirrorCore.Lambda.StrongFoldApp.
+
+Set Implicit Arguments.
+Set Strict Implicit.
+
+(** NOTE: This could work on arbitrary expr's **)
+Section seplog_fold.
+  Variable typ : Type.
+  Variable RType_typ : RType typ.
+  Variable Typ2_Fun : Typ2 _ Fun.
+  Variable sym : Type.
+  Variable RSym_sym : RSym sym.
+
+  Let tyArr : typ -> typ -> typ := @typ2 _ _ _ _.
+
+  Let Expr_expr := @Expr_expr typ sym _ _ _.
+  Local Existing Instance Expr_expr.
+
+  Variable T : Type.
+  Variable SL : typ.
+
+  Record SepLogArgs : Type :=
+  { do_other : expr typ sym -> list (expr typ sym * T) -> T
+  ; do_pure : expr typ sym -> T
+  ; do_emp : T
+  ; do_star : T -> T -> T
+  ; do_and : T -> T -> T
+  ; do_ex : typ -> T -> T
+  }.
+
+  Record SepLogSpec : Type :=
+  { is_pure : expr typ sym -> bool
+  ; is_emp : expr typ sym -> bool
+  ; is_star : expr typ sym -> bool
+  ; is_and : expr typ sym -> bool
+  ; is_ex : expr typ sym -> option typ
+  }.
+
+  Variable sla : SepLogArgs.
+  Variable sls : SepLogSpec.
+
+  Record SepLogSpecOk (sls : SepLogSpec)
+         (OPS : ILogic.ILogicOps (typD nil SL))
+         (BI : BILOperators (typD nil SL)) : Type :=
+  { _PureOp : @PureOp (typD nil SL)
+  ; _Pure : @Pure _ OPS BI _PureOp
+  ; His_pure : forall e,
+                 sls.(is_pure) e = true ->
+                 forall us vs val,
+                   exprD us vs e SL = Some val ->
+                   pure val
+  ; His_emp : forall e,
+                sls.(is_emp) e = true ->
+                forall us vs,
+                  exprD us vs e SL = Some empSP
+  ; His_star : forall e,
+                 sls.(is_star) e = true ->
+                 forall us vs,
+                   exprD us vs e (tyArr SL (tyArr SL SL)) =
+                   Some match eq_sym (typ2_cast nil SL (tyArr SL SL)) in _ = t
+                              return t
+                        with
+                          | eq_refl =>
+                            match eq_sym (typ2_cast nil SL SL) in _ = t
+                                  return _ -> t
+                            with
+                              | eq_refl => sepSP
+                            end
+                        end
+  }.
+
+  Record SepLogArgsOk (R_t : expr typ sym -> T -> tenv typ -> tenv typ -> Prop) :=
+  { otherOk
+    : forall ts e es tus tvs,
+        @typeof_apps typ sym _ _ _ ts tus tvs e (List.map fst es) = Some SL ->
+        (forall x y,
+           In (x,y) es ->
+           typeof_expr ts tus tvs x = Some SL ->
+           R_t x y tus tvs) ->
+        R_t (apps e (List.map fst es)) (sla.(do_other) e es) tus tvs
+  ; pureOk
+    : forall ts e tus tvs,
+        typeof_expr ts tus tvs e = Some SL ->
+        sls.(is_pure) e = true ->
+        R_t e (sla.(do_pure) e) tus tvs
+  ; empOk
+    : forall e tus tvs,
+        typeof_sym e = Some SL ->
+        sls.(is_emp) (Inj e) = true ->
+        R_t (Inj e) sla.(do_emp) tus tvs
+  ; starOk
+    : forall ts e l r l_res r_res tus tvs,
+        typeof_sym e = Some (tyArr SL (tyArr SL SL)) ->
+        typeof_expr ts tus tvs l = Some SL ->
+        typeof_expr ts tus tvs r = Some SL ->
+        sls.(is_star) (Inj e) = true ->
+        R_t l l_res tus tvs ->
+        R_t r r_res tus tvs ->
+        R_t (apps (Inj e) (l :: r :: nil)) (sla.(do_star) l_res r_res) tus tvs
+  }.
+
+  Require Import ExtLib.Structures.Applicative.
+  Instance Applicative_Lazy : Applicative Lazy :=
+  { ap := fun _ _ f x z => (f z) (x z)
+  ; pure := fun _ x => fun _ => x }.
+
+  Definition AppFullFoldArgs_SepLogArgs
+  : @AppFullArgs typ sym (fun x => T).
+  refine
+    match sla , sls with
+      | {| do_other := do_other
+         ; do_pure := do_pure
+         ; do_star := do_star
+         ; do_and := do_and
+         ; do_emp := do_emp
+         ; do_ex := do_ex |}
+      , {| is_pure := is_pure
+         ; is_star := is_star
+         ; is_and := is_and
+         ; is_emp := is_emp
+         ; is_ex := is_ex |} =>
+        @Build_AppFullArgs typ sym (fun x => T)
+          (fun v _ =>
+             if is_pure (Var v) then
+               do_pure (Var v)
+             else
+               if is_emp (Var v) then
+                 do_emp
+               else
+                 do_other (Var v) nil)
+          (fun u _ =>
+             if is_pure (UVar u) then
+               do_pure (UVar u)
+             else
+               if is_emp (UVar u) then
+                 do_emp
+               else
+                 do_other (UVar u) nil)
+          (fun i _ =>
+             if is_emp (Inj i) then
+               do_emp
+             else
+               if is_pure (Inj i) then
+                 do_pure (Inj i)
+               else
+                 do_other (Inj i) nil)
+          (fun f fres args rec =>
+             if is_star f then
+               match args as args
+                     return Lazy T
+               with
+                 | (existT _ l) :: (existT _ r) :: nil =>
+                   fun _ => do_star (l tt) (r tt)
+                 | _ => fun _ => do_emp
+               end
+             else if is_and f then
+                    match args as args
+                          return Lazy T
+                    with
+                      | (existT _ l) :: (existT _ r) :: nil =>
+                        fun _ => do_and (l tt) (r tt)
+                      | _ => fun _ => do_emp
+                    end
+                  else
+                    match is_ex f with
+                      | Some t =>
+                        match args as args return
+                              (forall y, TransitiveClosure.rightTrans (@expr_acc _ _) y
+                                                    (apps f (map (@projT1 _ _) args)) -> T) ->
+                              Lazy T
+                        with
+                          | existT (Abs _ e') _ :: nil =>
+                            fun rec _ => do_ex t (@rec e' _)
+                          | _ => fun _ =>
+                            let original := apps f (map (@projT1 _ _) args) in
+                            if is_pure original then
+                              fun _ => do_pure original
+                            else
+                              fun _ =>
+                                do_other f (map (fun (e_es : {e : expr typ sym & Lazy T }) =>
+                                                   match e_es
+                                                         return expr typ sym * T with
+                                                     | existT e es =>
+                                                       (e, es tt)
+                                                   end) args)
+                        end rec
+                      | None =>
+                        let original := apps f (map (@projT1 _ _) args) in
+                        if is_pure original then
+                          fun _ => do_pure original
+                        else
+                          fun _ =>
+                            do_other f (map (fun (e_es : {e : expr typ sym & Lazy T }) =>
+                                               match e_es
+                                                     return expr typ sym * T with
+                                                 | existT e es =>
+                                                   (e, es tt)
+                                               end) args)
+                    end)
+          (fun t e eres rec =>
+             if is_pure (Abs t e) then
+               fun _ => do_pure (Abs t e)
+             else
+               if is_emp (Abs t e) then
+                 fun _ => do_emp
+               else
+                 fun _ => do_other (Abs t e) nil)
+    end.
+  simpl.
+  eapply TransitiveClosure.RTStep.
+  eapply TransitiveClosure.RTFin.
+  apply acc_Abs. eapply acc_App_r.
+  Defined.
+
+(* TODO(gmalecha): Port the proof!
+  Section sound.
+    Hypothesis BILOps : BILOperators (typD nil SL).
+    Context R_t `{slaok : SepLogArgsOk R_t}.
+
+    Lemma atomic_ok
+    : forall ts (tus tvs : tenv typ) e (t : typ),
+        typeof_expr ts tus tvs e = Some t ->
+        t = SL ->
+        R_t e (sla.(do_other) e nil) tus tvs.
+    Proof.
+      destruct slaok. simpl; intros. subst.
+      change e with (apps e nil) at 1.
+      eapply (otherOk0 ts e nil tus tvs); simpl.
+      { unfold typeof_apps. simpl. rewrite H. reflexivity. }
+      { intuition. }
+    Qed.
+
+    Hypothesis is_starOk
+    : forall i,
+        sls.(is_star) (Inj i) = true ->
+        typeof_sym i = Some (tyArr SL (tyArr SL SL)).
+
+    Lemma lem_other
+    : forall ts0 t rs tus tvs l_res do_atomic_app0,
+        Forall2
+          (fun (t0 : typ) (x : expr sym * (tenv typ -> tenv typ -> T)) =>
+             typeof_expr tus tvs (fst x) = Some t0 /\
+             (t0 = SL -> R_t (fst x) (snd x tus tvs) tus tvs)) ts0 rs ->
+        forall e : expr sym,
+          typeof_expr tus tvs (apps e (map fst rs)) = Some t ->
+          (fold_right tyArr t ts0 = SL -> R_t e (l_res tus tvs) tus tvs) ->
+          typeof_apps RSym_sym tus tvs e (map fst rs) = Some SL ->
+          (forall (e0 : expr sym) (es : list (expr sym * T)) (tus0 tvs0 : tenv typ),
+             typeof_apps RSym_sym tus0 tvs0 e0 (map fst es) = Some SL ->
+             (forall (x : expr sym) (y : T),
+                In (x, y) es -> typeof_expr tus0 tvs0 x = Some SL -> R_t x y tus0 tvs0) ->
+             R_t (apps e0 (map fst es)) (do_atomic_app0 e0 es) tus0 tvs0) ->
+          R_t (apps e (map fst rs))
+              (do_atomic_app0 e
+                              (map
+                                 (fun x : expr sym * (tenv typ -> tenv typ -> T) =>
+                                    (fst x, snd x tus tvs)) rs)) tus tvs.
+    Proof.
+      intros.
+      specialize (H3 e (map
+                          (fun x : expr sym * (tenv typ -> tenv typ -> T) =>
+                             (fst x, snd x tus tvs)) rs) tus tvs).
+      rewrite map_map in *. simpl in *.
+      eapply H3; eauto.
+      clear - H. induction H; simpl; intuition.
+      inv_all. subst. rewrite H1 in *. inv_all; subst.
+      eauto.
+    Qed.
+
+    Definition AppFullFoldArgsOk_SepLogsOk
+    : AppFullFoldArgsOk _ (AppFullFoldArgs_SepLogArgs sla)
+                        (fun t e res tus tvs =>
+                           t = SL ->
+                           R_t e res tus tvs).
+    Proof.
+      remember sla as s; destruct s; simpl; remember sls as s; destruct s.
+      constructor.
+      { simpl; intros.
+        replace do_other0 with (sla.(do_other)).
+        eapply atomic_ok; eauto. rewrite <- Heqs; reflexivity. }
+      { simpl; intros.
+        replace do_other0 with (sla.(do_other)).
+        eapply atomic_ok; eauto. rewrite <- Heqs; reflexivity. }
+      { simpl; intros.
+        consider (is_emp0 v); intros.
+        { replace do_emp0 with (sla.(do_emp)).
+          eapply (@empOk _ slaok); eauto.
+          Cases.rewrite_all_goal. auto.
+          rewrite <- Heqs0. simpl. auto.
+          rewrite <- Heqs. reflexivity. }
+        { replace do_other0 with (sla.(do_other)).
+          eapply atomic_ok; eauto. rewrite <- Heqs; reflexivity. } }
+      { simpl; intros.
+        replace do_other0 with (sla.(do_other)).
+        eapply atomic_ok; eauto. rewrite <- Heqs; reflexivity. }
+      { intros. subst ft. simpl.
+        assert (typeof_apps RSym_sym tus tvs l (map fst rs) = Some SL).
+        { rewrite <- typeof_expr_apps. congruence. }
+        generalize (otherOk slaok). rewrite <- Heqs. simpl.
+        destruct l; eauto using lem_other.
+        consider (is_star0 s); eauto using lem_other; intros.
+        { generalize H4. eapply is_starOk in H4.
+          unfold typeof_apps in H3.
+          simpl in H3. rewrite H4 in *.
+          inversion H1; clear H1; try subst.
+          { subst rs ts0; intros.
+            simpl in *. clear - H3. inv_all.
+            symmetry in H3. eapply tyArr_circ_L in H3. intuition. }
+          { subst rs ts0. inversion H7; clear H7.
+            { subst l l'; intros; simpl in *.
+              rewrite H4 in *. forward.
+              intuition. inv_all. subst y t0.
+              clear - H8. symmetry in H8.
+              eapply tyArr_circ_L in H8. intuition. }
+            { subst l l'. inversion H8; clear H8.
+              { subst l0 l'0. intuition. subst t.
+                destruct y, y0; simpl in *.
+                rewrite H8 in *. rewrite H6 in *. rewrite H4 in *.
+                unfold type_of_apply in *. forward.
+                inv_all.
+                subst x0 x t1 t2 t3 p0 p.
+                replace do_star0 with (sla.(do_star));
+                  [ | rewrite <- Heqs; reflexivity ].
+                eapply (starOk slaok); eauto.
+                rewrite <- Heqs0. auto. }
+              { exfalso. clear Heqs Heqs0. subst.
+                simpl in H3. intuition.
+                rewrite H2 in *. rewrite H6 in *. rewrite H1 in *.
+                forward. inv_all; try subst.
+                clear H15 H13. subst x x0 x1.
+                clear - H14.
+                eapply type_of_applys_circle_False in H14. auto. } } } } }
+    Qed.
+
+    Definition seplog_fold (sla : SepLogArgs) : expr sym -> tenv typ -> tenv typ -> T :=
+      app_fold_args (AppFullFoldArgs_SepLogArgs sla).
+
+    Theorem seplog_fold_sound
+    : forall e tus tvs result,
+        seplog_fold sla e tus tvs = result ->
+        typeof_expr tus tvs e = Some SL ->
+        R_t e result tus tvs.
+    Proof.
+      intros.
+      eapply (app_fold_args_sound AppFullFoldArgsOk_SepLogsOk) in H; eauto.
+    Qed.
+  End sound.
+*)
+
+
+(*
+  Variable OPS : ILogic.ILogicOps (typD ts nil SL).
+  Variable BI : BILOperators (typD ts nil SL).
+  Variable slsok : SepLogSpecOk sls OPS BI.
+
+  Require Import Relations.
+  Require Import ExtLib.Data.HList.
+
+  Record SepLogArgsSemOk
+         (TD : T -> forall tus tvs, tenv typ -> tenv typ -> option (typD ts nil SL))
+         (R : forall tus tvs,
+                relation (hlist (typD ts nil) tus ->
+                          hlist (typD ts nil) tvs ->
+                          typD ts nil SL)) :=
+  { atomic_appOk
+    : forall e es tus tvs val,
+        exprD' tus tvs (apps e es) SL = Some val ->
+        R tus tvs val (TD (sla.(do_other) e es))
+  ; pureOk
+    : forall e tus tvs,
+        typeof_expr tus tvs e = Some SL ->
+        sls.(is_pure) e = true ->
+        R_t e (sla.(do_pure) e) tus tvs
+  ; empOk
+    : forall e tus tvs,
+        typeof_sym e = Some SL ->
+        sls.(is_emp) e = true ->
+        R_t (Inj e) sla.(do_emp) tus tvs
+  ; starOk
+    : forall e l r l_res r_res tus tvs,
+        typeof_sym e = Some (tyArr SL (tyArr SL SL)) ->
+        typeof_expr tus tvs l = Some SL ->
+        typeof_expr tus tvs r = Some SL ->
+        sls.(is_star) e = true ->
+        R_t l l_res tus tvs ->
+        R_t r r_res tus tvs ->
+        R_t (apps (Inj e) (l :: r :: nil)) (sla.(do_star) l_res r_res) tus tvs
+  }.
+*)
+
+End seplog_fold.
